work towards r2a

dimsum/iris/expr2.v
@@ -26,8 +26,8 @@ Global Arguments mexpr_rel {_ _} _ _ _.
 Global Arguments mstate_interp {_ _} _ _.
 
 Definition switch `{!dimsumGS Σ} {S EV} (Π : option EV → S → iProp Σ)
-  (K : option EV → S → (tgt_src → ∀ m : mod_trans EV, _ → iProp Σ) → iProp Σ) : iProp Σ :=
-  (∀ κ σ, K κ σ (λ ts' m' PΠ', ∀ σ' Π', PΠ' σ' Π' -∗ σ' ≈{ ts', m' }≈> Π') -∗  Π κ σ).
+  (K : option EV → S → (tgt_src → ∀ EV2, ∀ m : mod_trans EV2, _ → iProp Σ) → iProp Σ) : iProp Σ :=
+  (∀ κ σ, K κ σ (λ ts' EV2 m' PΠ', ∀ σ' Π', PΠ' σ' Π' -∗ σ' ≈{ ts', m' }≈> Π') -∗  Π κ σ).
 
 (* Lemma switch_mono `{!dimsumGS Σ} {S EV} (Π : option EV → S → iProp Σ) K1 K2 : *)
 (*   switch Π K1 -∗ *)
@@ -43,7 +43,7 @@ Definition switch_id `{!dimsumGS Σ} {EV} (ts : tgt_src) (m : mod_trans EV)
   (Π : option EV → m.(m_state) → iProp Σ)
   (κ : option EV) (σ : m.(m_state)) (C : m.(m_state) → iProp Σ) : iProp Σ :=
   switch Π ({{ κs σs POST, ⌜κs = κ⌝ ∗ ⌜σs = σ⌝ ∗
-  POST ts m ({{ σ' Πs, ⌜Πs = Π⌝ ∗ C σ'}})}})%I.
+  POST ts _ m ({{ σ' Πs, ⌜Πs = Π⌝ ∗ C σ'}})}})%I.
 
 Lemma switch_id_mono `{!dimsumGS Σ} {EV} ts (m : mod_trans EV)
   (Π : option EV → m.(m_state) → iProp Σ) κ σ C1 C2 :
@@ -62,11 +62,11 @@ Definition switch_external `{!dimsumGS Σ} {S EV} (Π : option EV → S → iPro
   (K : _) : iProp Σ :=
   switch Π ({{ κ σ POST,
     K κ σ ({{ m2 σ2 K2,
-  POST Src m2 ({{ σ_s Π_s,
+  POST Src _ m2 ({{ σ_s Π_s,
     ⌜σ_s = σ2⌝ ∗
   switch Π_s ({{ κ' σ_s2 POST,
     ⌜κ' = κ⌝ ∗
-  POST Src _ ({{ σ_s2' Π',
+  POST Src _ _ ({{ σ_s2' Π',
     ⌜σ_s2' = σ_s2⌝ ∗ K2 σ_s2 Π'}})}})}})}})}})%I.
 
 (* Switching to a linked module *)
@@ -74,11 +74,11 @@ Definition switch_link `{!dimsumGS Σ} {S EV} (ts : tgt_src) (Π : option (io_ev
   (K : _) : iProp Σ :=
   switch Π ({{ κ σ0 POST,
     K σ0 ({{ e m2 σ2 K2, ⌜κ = Some (Outgoing, e)⌝ ∗
-  POST ts m2 ({{ σi Πi,
+  POST ts _ m2 ({{ σi Πi,
     ⌜σi = σ2⌝ ∗
   switch Πi ({{ κ' σ POST,
     ∃ e', ⌜κ' = Some (Incoming, e')⌝ ∗
-  POST ts m2 ({{ σr Πr,
+  POST ts _ m2 ({{ σr Πr,
     ⌜σr = σ⌝ ∗ ⌜e' = e⌝ ∗ K2 σ Πr}})}})}})}})}})%I.
 
 
